Leanbin/Init/Control/Lift.lean
@@ -55,9 +55,9 @@ theorem monad_lift_refl {m : Type u → Type v} {α} : (monadLift : m α → m �
 
 /- warning: monad_functor -> MonadFunctor is a dubious translation:
 lean 3 declaration is
-  (Type.{u} -> Type.{v}) -> (Type.{u} -> Type.{v}) -> (Type.{u} -> Type.{w}) -> (Type.{u} -> Type.{w}) -> Sort.{max (succ (succ u)) (succ v) (succ w)}
+  (Type.{u1} -> Type.{u2}) -> (Type.{u1} -> Type.{u2}) -> (Type.{u1} -> Type.{u3}) -> (Type.{u1} -> Type.{u3}) -> Sort.{max (succ (succ u1)) (succ u2) (succ u3)}
 but is expected to have type
-  (Type.{u} -> Type.{v}) -> (Type.{u} -> Type.{w}) -> Sort.{max (max (succ (succ u)) (succ v)) (succ w)}
+  (Type.{u1} -> Type.{u2}) -> (Type.{u1} -> Type.{u3}) -> Sort.{max (max (succ (succ u1)) (succ u2)) (succ u3)}
 Case conversion may be inaccurate. Consider using '#align monad_functor MonadFunctorₓ'. -/
 /-- A functor in the category of monads. Can be used to lift monad-transforming functions.
     Based on pipes' [MFunctor](https://hackage.haskell.org/package/pipes-2.4.0/docs/Control-MFunctor.html),
@@ -69,9 +69,9 @@ class MonadFunctor (m m' : Type u → Type v) (n n' : Type u → Type w) where
 
 /- warning: monad_functor_t -> MonadFunctorT is a dubious translation:
 lean 3 declaration is
-  (Type.{u} -> Type.{v}) -> (Type.{u} -> Type.{v}) -> (Type.{u} -> Type.{w}) -> (Type.{u} -> Type.{w}) -> Sort.{max (succ (succ u)) (succ v) (succ w)}
+  (Type.{u1} -> Type.{u2}) -> (Type.{u1} -> Type.{u2}) -> (Type.{u1} -> Type.{u3}) -> (Type.{u1} -> Type.{u3}) -> Sort.{max (succ (succ u1)) (succ u2) (succ u3)}
 but is expected to have type
-  (Type.{u} -> Type.{v}) -> (Type.{u} -> Type.{w}) -> Sort.{max (max (succ (succ u)) (succ v)) (succ w)}
+  (Type.{u1} -> Type.{u2}) -> (Type.{u1} -> Type.{u3}) -> Sort.{max (max (succ (succ u1)) (succ u2)) (succ u3)}
 Case conversion may be inaccurate. Consider using '#align monad_functor_t MonadFunctorTₓ'. -/
 /-- The reflexive-transitive closure of `monad_functor`.
     `monad_map` is used to transitively lift monad morphisms such as `state_t.zoom`.
