Leanbin/Init/Data/Int/Order.lean
@@ -1496,7 +1496,7 @@ theorem sign_eq_zero_iff_zero (a : ℤ) : sign a = 0 ↔ a = 0 :=
 lean 3 declaration is
   forall {a : Int} {b : Int}, (Eq.{1} Int (HMul.hMul.{0, 0, 0} Int Int Int (instHMul.{0} Int Int.hasMul) a b) (OfNat.ofNat.{0} Int 0 (OfNat.mk.{0} Int 0 (Zero.zero.{0} Int Int.hasZero)))) -> (Or (Eq.{1} Int a (OfNat.ofNat.{0} Int 0 (OfNat.mk.{0} Int 0 (Zero.zero.{0} Int Int.hasZero)))) (Eq.{1} Int b (OfNat.ofNat.{0} Int 0 (OfNat.mk.{0} Int 0 (Zero.zero.{0} Int Int.hasZero)))))
 but is expected to have type
-  forall {n : Nat} {m : Nat}, (Eq.{1} Nat (HMul.hMul.{0, 0, 0} Nat Nat Nat (instHMul.{0} Nat instMulNat) n m) (OfNat.ofNat.{0} Nat 0 (instOfNatNat 0))) -> (Or (Eq.{1} Nat n (OfNat.ofNat.{0} Nat 0 (instOfNatNat 0))) (Eq.{1} Nat m (OfNat.ofNat.{0} Nat 0 (instOfNatNat 0))))
+  forall {a : Nat} {b : Nat}, (Eq.{1} Nat (HMul.hMul.{0, 0, 0} Nat Nat Nat (instHMul.{0} Nat instMulNat) a b) (OfNat.ofNat.{0} Nat 0 (instOfNatNat 0))) -> (Or (Eq.{1} Nat a (OfNat.ofNat.{0} Nat 0 (instOfNatNat 0))) (Eq.{1} Nat b (OfNat.ofNat.{0} Nat 0 (instOfNatNat 0))))
 Case conversion may be inaccurate. Consider using '#align int.eq_zero_or_eq_zero_of_mul_eq_zero Int.eq_zero_or_eq_zero_of_mul_eq_zeroₓ'. -/
 protected theorem eq_zero_or_eq_zero_of_mul_eq_zero {a b : ℤ} (h : a * b = 0) : a = 0 ∨ b = 0 :=
   match lt_trichotomy 0 a with
