Leanbin/Init/Function.lean
@@ -100,9 +100,9 @@ theorem right_id (f : α → β) : f ∘ id = f :=
 
 /- warning: function.comp_app -> Function.comp_apply is a dubious translation:
 lean 3 declaration is
-  forall {α : Sort.{u₁}} {β : Sort.{u₂}} {φ : Sort.{u₃}} (f : β -> φ) (g : α -> β) (a : α), Eq.{u₃} φ (Function.comp.{u₁, u₂, u₃} α β φ f g a) (f (g a))
+  forall {α : Sort.{u1}} {β : Sort.{u2}} {φ : Sort.{u3}} (f : β -> φ) (g : α -> β) (a : α), Eq.{u3} φ (Function.comp.{u1, u2, u3} α β φ f g a) (f (g a))
 but is expected to have type
-  forall {β : Sort.{u_1}} {δ : Sort.{u_2}} {α : Sort.{u_3}} {f : β -> δ} {g : α -> β} {x : α}, Eq.{u_2} δ (Function.comp.{u_3, u_1, u_2} α β δ f g x) (f (g x))
+  forall {α : Sort.{u3}} {β : Sort.{u2}} {φ : Sort.{u1}} {f : α -> β} {g : φ -> α} {a : φ}, Eq.{u2} β (Function.comp.{u1, u3, u2} φ α β f g a) (f (g a))
 Case conversion may be inaccurate. Consider using '#align function.comp_app Function.comp_applyₓ'. -/
 @[simp]
 theorem comp_apply (f : β → φ) (g : α → β) (a : α) : (f ∘ g) a = f (g a) :=
