Leanbin/Init/Meta/Smt/Ematch.lean
@@ -117,14 +117,16 @@ unsafe def to_hinst_lemmas_core (m : Transparency) :
 unsafe def mk_hinst_lemma_attr_core (attr_name : Name) (as_simp : Bool) : Tactic := do
   let t := q(user_attribute hinst_lemmas)
   let v :=
-    q(({ Name := attr_name, descr := "hinst_lemma attribute",
+    q(({  Name := attr_name
+          descr := "hinst_lemma attribute"
           after_set :=
             some fun n _ _ =>
               to_hinst_lemmas_core reducible as_simp [n] hinst_lemmas.mk >> skip <|>
-                fail f! "invalid ematch lemma '{n}'",-- allow unsetting
-          before_unset := some fun _ _ => skip,
+                fail f! "invalid ematch lemma '{n}'"
+          -- allow unsetting
+          before_unset := some fun _ _ => skip
           cache_cfg :=
-            { mk_cache := fun ns => to_hinst_lemmas_core reducible as_simp ns hinst_lemmas.mk,
+            { mk_cache := fun ns => to_hinst_lemmas_core reducible as_simp ns hinst_lemmas.mk
               dependencies := [`reducibility] } } :
         user_attribute hinst_lemmas))
   add_decl (declaration.defn attr_name [] t v ReducibilityHints.abbrev ff)
@@ -164,17 +166,19 @@ unsafe def mk_hinst_lemma_attr_set (attr_name : Name) (attr_names : List Name)
   mk_hinst_lemma_attrs_core tt simp_attr_names
   let t := q(user_attribute hinst_lemmas)
   let v :=
-    q(({ Name := attr_name, descr := "hinst_lemma attribute set",
+    q(({  Name := attr_name
+          descr := "hinst_lemma attribute set"
           after_set :=
             some fun n _ _ =>
               to_hinst_lemmas_core reducible false [n] hinst_lemmas.mk >> skip <|>
-                fail f! "invalid ematch lemma '{n}'",-- allow unsetting
-          before_unset := some fun _ _ => skip,
+                fail f! "invalid ematch lemma '{n}'"
+          -- allow unsetting
+          before_unset := some fun _ _ => skip
           cache_cfg :=
             { mk_cache := fun ns => do
                 let hs₁ ← to_hinst_lemmas_core reducible false ns hinst_lemmas.mk
                 let hs₂ ← merge_hinst_lemma_attrs reducible false attr_names hs₁
-                merge_hinst_lemma_attrs reducible tt simp_attr_names hs₂,
+                merge_hinst_lemma_attrs reducible tt simp_attr_names hs₂
               dependencies := [`reducibility] ++ attr_names ++ simp_attr_names } } :
         user_attribute hinst_lemmas))
   add_decl (declaration.defn attr_name [] t v ReducibilityHints.abbrev ff)
